Typecheck smallstep_monad (but temporarily admit proofs)

smallstep_monad.v
@@ -45,7 +45,7 @@ Next Obligation.
 destruct M2; reflexivity.
 Qed.
 
-Program Fixpoint denotation {A : Type} (p : program A) : M A :=
+Program Fixpoint denotation {A : Type} (p : program A) : MonadStateTrace.m M A :=
   match p with
   | p_ret _ v => Ret v
   | p_bind _ _ m f => do a <- denotation m; denotation (f a)
@@ -55,23 +55,31 @@ Program Fixpoint denotation {A : Type} (p : program A) : M A :=
   | p_mark t => Mark _ t
   end.
 
-Fixpoint denotation_continuation (k : continuation) : M (@continuation T S) :=
+Next Obligation.
+intros; exact M0.
+Defined.
+
+Next Obligation.
+intros; exact M0.
+Defined.
+
+Fixpoint denotation_continuation (k : continuation) :
+  MonadStateTrace.m M (@continuation T S) :=
   match k with
-  | stop A a => Ret (stop A a)
+  | stop A a => MonadStateful.ret M0 (stop A a)
   | p `; f =>
-      do a <- denotation p ;
-      denotation_continuation (f a)
+      MonadStateful.bind (M := M0) (denotation p) (fun a => denotation_continuation (f a))
   end.
 
-Definition stateTrace_sub {A : Type} (m : M A) : Type :=
+Definition stateTrace_sub {A : Type} (m : MonadStateTrace.m M A) : Type :=
   { p | denotation p = m }.
 
-Definition continuation_sub (m : M continuation) : Type :=
+Definition continuation_sub (m : MonadStateTrace.m M continuation) : Type :=
   {k | denotation_continuation k = m }.
 
-Lemma denotation_prefix_preserved A (m : M A) :
+Lemma denotation_prefix_preserved A (m : MonadStateTrace.m M A) :
   stateTrace_sub m -> forall s s' l1 l a,
-  Run m (s, l1) = (a, (s', l)) -> exists l2, l = l1 ++ l2.
+  Run (M := M0) m (s, l1) = (a, (s', l)) -> exists l2, l = l1 ++ l2.
 Proof.
 intros [ p Hp ].
 subst m.
@@ -79,6 +87,8 @@ induction p as [ A a | A B p IHp g IHg | A b p1 IHp1 p2 IHp2 | | s0 | t ]; cbn;
  intros s s' l1 l a' Heq.
 - exists [].
   rewrite app_nil_r.
+Admitted.
+(*
   by move: Heq; rewrite runret => -[].
 - rewrite runbind in Heq.
   case_eq (Run (denotation p) (s, l1)).
@@ -101,16 +111,19 @@ induction p as [ A a | A B p IHp g IHg | A b p1 IHp1 p2 IHp2 | | s0 | t ]; cbn;
 - exists [t].
   by move: Heq; rewrite runmark => -[].
 Qed.
+*)
 
-Lemma denotation_prefix_independent A (m : M A) :
+Lemma denotation_prefix_independent A (m : MonadStateTrace.m M A) :
   stateTrace_sub m -> forall s l1 l2,
-  Run m (s, l1 ++ l2) =
-  let res := Run m (s, l2) in
+  Run (M := M0) m (s, l1 ++ l2) =
+  let res := Run (M := M0) m (s, l2) in
   (res.1, (res.2.1, l1 ++ res.2.2)).
 Proof.
 intros [ p Hp ] s l1 l2.
 subst m.
 elim: p s l1 l2 => /= {A} [A a|A B p1 IH1 p2 IH2|A b p1 IH1 p2 IH2||s'|t] s l1 l2.
+Admitted.
+(*
 by rewrite !runret.
 rewrite [in LHS]runbind [in LHS]IH1.
 rewrite [in RHS]runbind.
@@ -121,26 +134,31 @@ by rewrite !runget.
 by rewrite !runput.
 by rewrite !runmark !seq.cats1 seq.rcons_cat.
 Qed.
+*)
 
 Lemma denotation_continuation_prefix_independent m :
   continuation_sub m -> forall s l1 l2,
-  Run m (s, l1 ++ l2) =
-  let res := Run m (s, l2) in
+  Run (M := M0) m (s, l1 ++ l2) =
+  let res := Run (M := M0) m (s, l2) in
   (res.1, (res.2.1, l1 ++ res.2.2)).
 Proof.
 intros [ k Hk ].
 subst m.
 elim: k => // [A a s l1 l2|A p k IH s l1 l2].
+Admitted.
+(*
 by rewrite !runret.
 rewrite /= !runbind.
 rewrite denotation_prefix_independent /=; [ | now exists p ].
 destruct (Run (denotation p) (s, l2)) as [ a (s', l) ].
 by rewrite IH.
 Qed.
+*)
 
 Lemma step_None_correct s s' k k' l :
   step (s, k) None (s', k') ->
-  Run (denotation_continuation k) (s, l) = Run (denotation_continuation k') (s', l).
+  Run (M := M0) (denotation_continuation k) (s, l) =
+  Run (M := M0) (denotation_continuation k') (s', l).
 Proof.
 intro Hstep.
 remember (s, k) as sk eqn: Heq.
@@ -151,6 +169,8 @@ induction Hstep as
  [ s A a f | s A B p f g | s A p1 p2 k | s A p1 p2 k | s f | s s' f | s t f ];
  intros s1 s2 k1 k2 l [= Hs1 Hk1] [= Hs2 Hk2] Heqo.
 - subst s1 k1 s2 k2.
+Admitted.
+(*
   by rewrite /= runbind runret.
 - subst s1 k1 s2 k2.
   cbn.
@@ -165,11 +185,12 @@ induction Hstep as
   by rewrite /= runbind runput.
 - discriminate Heqo.
 Qed.
+*)
 
 Lemma step_Some_correct s s' k k' t l :
   step (s, k) (Some t) (s', k') ->
-  Run (denotation_continuation k) (s, l) =
-  Run (denotation_continuation k') (s', l ++ [t]).
+  Run (M := M0) (denotation_continuation k) (s, l) =
+  Run (M := M0) (denotation_continuation k') (s', l ++ [t]).
 Proof.
 intro Hstep.
 remember (s, k) as sk eqn: Heq.
@@ -181,12 +202,16 @@ induction Hstep as
  intros s1 s2 k1 k2 l [= Hs1 Hk1] [= Hs2 Hk2] Heqo; try discriminate Heqo.
 subst s1 k1 s2 k2.
 injection Heqo; intro; subst t.
+Admitted.
+(*
 by rewrite /= runbind runmark.
 Qed.
+*)
 
 Lemma step_star_correct_gen s s' k k' l l' :
   step_star (s, k) l' (s', k') ->
-  Run (denotation_continuation k) (s, l) = Run (denotation_continuation k') (s', l++l').
+  Run (M := M0) (denotation_continuation k) (s, l) =
+  Run (M := M0) (denotation_continuation k') (s', l++l').
 Proof.
 intro Hstep_star.
 remember (s, k) as sk eqn: Heq.
@@ -220,11 +245,13 @@ Qed.
 Proposition step_star_correct
   (s s' : S) (A : Type) (a : A) (p : program A) (l : list T) :
   step_star (s, p `; stop A) l (s', stop A a) ->
-  Run (denotation p) (s, []) = (a, (s', l)).
+  Run (M := M0) (denotation p) (s, []) = (a, (s', l)).
 Proof.
 intro Hss.
 apply step_star_correct_gen with (l := []) in Hss.
 move: Hss.
+Admitted.
+(*
 rewrite /= runret runbind.
 destruct (Run (denotation p) (s, [])) as [a'' [s'' l'']].
 rewrite runret => Hss.
@@ -232,15 +259,18 @@ injection Hss; clear Hss; intros Heq1 Heq2 Heq3.
 apply inj_pair2 in Heq3.
 congruence.
 Qed.
+*)
 
 Lemma step_star_complete_gen
   (s s' : S) (A : Type) (a : A) (p : program A) (l1 l2 : list T) f :
-  Run (denotation p) (s, l1) = (a, (s', l1 ++ l2)) ->
+  Run (M := M0) (denotation p) (s, l1) = (a, (s', l1 ++ l2)) ->
   step_star (s, p `; f) l2 (s', f a).
 Proof.
 revert s s' a l1 l2 f.
 induction p as [ A a | A B p IHp g IHg | A b p1 IHp1 p2 IHp2 | |  aa | t ]; cbn;
  intros s s' a' l1 l2 f Heq.
+Admitted.
+(*
 - rewrite runret in Heq.
   injection Heq; clear Heq; intros; subst a' s'.
   replace l2 with (@nil T) by
@@ -293,10 +323,11 @@ induction p as [ A a | A B p IHp g IHg | A b p1 IHp1 p2 IHp2 | |  aa | t ]; cbn;
    (revert l2 H; induction l1; [ tauto | intros ? [=]; firstorder ]).
   eapply ss_step_Some; [ apply s_mark | apply ss_refl ].
 Qed.
+*)
 
 Proposition step_star_complete
   (s s' : S) (A : Type) (a : A) (p : program A) (l : list T) :
-  Run (denotation p) (s, []) = (a, (s', l)) ->
+  Run (M := M0) (denotation p) (s, []) = (a, (s', l)) ->
   step_star (s, p `; stop A) l (s', stop A a).
 Proof.
 intro Hp.
@@ -306,4 +337,4 @@ Qed.
 
 End DenotationalSemantics.
 
-Arguments denotation [T] [S] _ _.
+Arguments denotation [S] [T] _ _.
